extraction and cli for context interpreter

src/execute.ml
@@ -140,7 +140,7 @@ let repl verbosity sies (name : string) =
       else (Printf.sprintf "unknown command" |> print_endline; pure cfg))
     |> (fun cb -> user_input "> " cb cfg0)
 
-let interpret verbosity error_code_on_crash sies name fuel =
+let interpret verbosity error_code_on_crash sies (name: string) fuel =
   let print_step_header gen =
     debug_info verbosity intermediate ~style:bold
       (fun () -> Printf.sprintf "step %d:\n" gen) in
@@ -193,6 +193,7 @@ let interpret verbosity error_code_on_crash sies name fuel =
         | None -> eval_cfg (gen + 1) ((((hs', s'), vs'), es)) max_steps
         end) in
 
+  debug_info verbosity result ~style:yellow (fun _ -> "Context optimisation disabled\n");
   print_step_header 0 ;
   debug_info verbosity intermediate (fun _ ->
     Printf.sprintf "\n%s\n" (pp_config_tuple_except_store (tuple_drop_hs cfg0)));
@@ -204,7 +205,106 @@ let interpret verbosity error_code_on_crash sies name fuel =
   if error_code_on_crash && (match res with None -> true | Some _ -> false) then exit 1
   else pure ()
 
-let instantiate_interpret verbosity interactive error_code_on_crash m name fuel =
+  (*
+module Interpreter_ctx_extract :
+ sig
+  val host_application_impl :
+    Equality.sort -> EmptyHost.store_record -> function_type -> Equality.sort
+    -> value list -> Equality.sort * (EmptyHost.store_record * result) option
+
+  val run_one_step_ctx : Equality.sort -> cfg_tuple_ctx -> run_step_ctx_result
+
+  val run_step_cfg_ctx_reform : cfg_tuple_ctx -> cfg_tuple_ctx option
+
+  val run_v_init :
+    Equality.sort store_record -> administrative_instruction list ->
+    cfg_tuple_ctx option
+
+  val es_of_cfg : cfg_tuple_ctx -> administrative_instruction list
+ end
+ *)
+
+include Extract.Interpreter_ctx_extract
+
+  let interpret_ctx verbosity error_code_on_crash sies (name: string) fuel =
+    let print_step_header gen =
+      debug_info verbosity intermediate ~style:bold
+        (fun () -> Printf.sprintf "step %d:\n" gen) in
+    let print_exhaustion gen = 
+      debug_info verbosity intermediate ~style:bold
+        (fun () -> Printf.sprintf "step %d: \n Execution halted due to fuel exhaustion\n" gen) in
+    let* cfg0 =
+      TopHost.from_out (
+        ovpending verbosity stage "interpreting" (fun _ ->
+          match lookup_exported_function name sies with
+          | None -> Error ("unknown function `" ^ name ^ "`")
+          | Some cfg0 -> OK cfg0)) in
+    let rec eval_cfg gen (hs: Extract.Equality.sort) (cfg: Extract.cfg_tuple_ctx) max_steps =
+      if (gen >= max_steps) then 
+        (print_exhaustion gen;
+        debug_info verbosity result ~style:bold (fun _ -> "fuel exhaustion\n");
+        pure None)
+      else 
+        (let run_step_res = run_one_step_ctx hs cfg in
+        print_step_header gen ;
+        match run_step_res with
+        | Extract.RSC_error _ ->
+          wait_message verbosity;
+          debug_info verbosity result ~style:red (fun _ -> "crash_error\n");
+          pure None
+        | Extract.RSC_admit ->
+          wait_message verbosity;
+          debug_info verbosity result ~style:red (fun _ -> "crash_admit\n");
+          pure None
+        | Extract.RSC_invalid ->
+          wait_message verbosity;
+          debug_info verbosity result ~style:red (fun _ -> "crash_invalid\n");
+          pure None
+        | Extract.RSC_value vs ->
+          debug_info verbosity result ~style:green (fun _ -> "success\n");
+          pure (Some vs)
+        | Extract.RSC_normal (hs_res, cfg_res) ->
+          debug_info verbosity intermediate
+          (fun () -> pp_es (es_of_cfg cfg_res)); 
+          debug_info verbosity intermediate
+          (fun () -> 
+            let (((s, _), _), _) = cfg in
+            let (((s', _), _), _) = cfg_res in 
+            let store_status = if s = s' then "unchanged" else "changed" in
+              Printf.sprintf "and store %s\n" store_status
+            ); 
+          debug_info verbosity store
+          (fun () ->
+            let (((s', _), _), _) = cfg_res in
+              Printf.sprintf "and store\n%s" (pp_store 1 s'));
+          (match run_step_cfg_ctx_reform cfg_res with
+          | Some cfg_res' -> eval_cfg (gen + 1) hs_res cfg_res' max_steps
+          | None -> pure None
+          )
+        ) in
+    debug_info verbosity result ~style:green (fun _ -> "Context optimisation on!\n");
+    print_step_header 0 ;
+
+    let (((hs, s), _), es) = cfg0 in
+    debug_info verbosity intermediate
+    (fun () -> pp_es es); 
+
+    let cfg_init = run_v_init s es in
+    (match cfg_init with
+    | Some cfg_init' ->
+      let* res = eval_cfg 0 hs cfg_init' fuel in
+      (debug_info_span verbosity result stage (fun _ ->
+        match res with
+        | Some vs -> pp_values vs
+        | None -> ""
+        );
+        if error_code_on_crash && (match res with None -> true | Some _ -> false) then exit 1
+        else pure ()
+      )
+    | None -> debug_info verbosity result ~style:red (fun _ -> "invalid starting es\n"); exit 1
+    )
+
+let instantiate_interpret verbosity interactive no_ctx_optimise error_code_on_crash m name fuel =
   let* store_inst_exps =
     TopHost.from_out (
       ovpending verbosity stage "instantiation" (fun _ ->
@@ -212,5 +312,5 @@ let instantiate_interpret verbosity interactive error_code_on_crash m name fuel 
         | None -> Error "instantiation error"
         | Some (store_inst_exps, _) -> OK store_inst_exps)) in
   if interactive then repl verbosity store_inst_exps name
-  else interpret verbosity error_code_on_crash store_inst_exps name fuel
-
+  else if no_ctx_optimise then interpret verbosity error_code_on_crash store_inst_exps name fuel
+  else interpret_ctx verbosity error_code_on_crash store_inst_exps name fuel
