theories/pp.v
@@ -11,10 +11,15 @@ Require Import ansi list_extra.
 Open Scope string_scope.
 
 Section Host.
-  
-Import Interpreter_func_extract.
 
+  (*
+Import Interpreter_func_extract.
+   *)
+
+Variable host_function: eqType.
+  
 Variable show_host_function : host_function -> string.
+
 
 Definition newline_char : Ascii.ascii := Ascii.ascii_of_byte Byte.x0a.
 
@@ -328,7 +333,7 @@ Fixpoint pp_basic_instruction (i : indentation) (be : basic_instruction) : strin
 Definition pp_basic_instructions n bes :=
   String.concat "" (List.map (pp_basic_instruction n) bes).
 
-Definition pp_function_closure (n : indentation) (fc : function_closure) : string :=
+Definition pp_function_closure (n : indentation) (fc : function_closure host_function) : string :=
   match fc with
   | FC_func_native i ft vs bes =>
     (* TODO: show instance? *)
@@ -401,7 +406,7 @@ Definition pp_table (n: indentation) (t : tableinst) : string :=
 Definition pp_tables (n : indentation) (ms : list tableinst) : string :=
   String.concat "" (mapi (fun i t => indent n (string_of_nat i ++ ": " ++ pp_table n t)) ms).
 
-Definition pp_store (n : indentation) (s : store_record) : string :=
+Definition pp_store (n : indentation) (s : store_record host_function) : string :=
   indent n ("globals" ++ newline) ++
   pp_globals (n.+1) s.(s_globals) ++
   indent n ("memories" ++ newline) ++
@@ -410,12 +415,12 @@ Definition pp_store (n : indentation) (s : store_record) : string :=
   pp_tables (n.+1) s.(s_tables).
 
 (* XXX disambiguate between cfg/res tuple with/without hs? *)
-Definition pp_config_tuple_except_store (cfg : store_record * frame * list administrative_instruction) : string :=
+Definition pp_config_tuple_except_store (cfg : store_record host_function * frame * list administrative_instruction) : string :=
   let '(s, f, es) := cfg in
   pp_administrative_instructions 0 es ++
   "with values " ++ pp_values_hint_empty f.(f_locs) ++ newline.
 
-Definition pp_res_tuple_except_store (res_cfg : store_record * frame * res_step) : string :=
+Definition pp_res_tuple_except_store (res_cfg : store_record host_function * frame * res_step) : string :=
   let '(s, f, res) := res_cfg in
   match res with
   | RS_crash _ =>
@@ -445,13 +450,16 @@ Section Show.
 
 Definition pp_values : list value -> string := pp_values.
 
-Definition pp_store : nat -> store_record -> string := pp_store.
+Definition pp_store : nat -> store_record -> string := pp_store host_function_eqType.
 
 Definition pp_res_tuple_except_store : store_record * frame * res_step -> string :=
-  pp_res_tuple_except_store.
+  pp_res_tuple_except_store host_function_eqType.
 
 Definition pp_config_tuple_except_store : store_record * frame * list administrative_instruction -> string :=
-  pp_config_tuple_except_store.
+  pp_config_tuple_except_store host_function_eqType.
+
+Definition pp_administrative_instructions : nat -> list administrative_instruction -> string :=
+  pp_administrative_instructions.
 
 End Show.
 
